Semantics/Imp/Aexp.lean
@@ -20,13 +20,11 @@ private instance equiv: Setoid Aexp where
   iseqv := {
     refl := fun _ => rfl
     symm := (Eq.symm .)
-    trans := (Eq.rec . .)
+    trans := (. ▸ .)
   }
 
 private example: ((var "x" + 5) + (9 - 7), s0) ==> 7 :=
-  BigStep.add
-    (BigStep.add BigStep.var BigStep.val)
-    (BigStep.sub BigStep.val BigStep.val)
+  .add (.add .var .val) (.sub .val .val)
 
 end BigStep
 
@@ -44,11 +42,11 @@ instance reduce.equiv: Setoid Aexp where
   r a a' := ∀{s}, a s = a' s
   iseqv := {
     refl := fun _ => rfl
-    symm := fun h => h.symm
-    trans := fun h1 h2 => h2.rec h1
+    symm := (Eq.symm .)
+    trans := (. ▸ .)
   }
 
-#eval ((var "x" + 5) + (9 - 7)) s0 -- 7
+#eval (var "x" + 5) + (9 - 7) $ s0 -- 7
 
 section Equivalence
 
@@ -56,22 +54,22 @@ section Equivalence
 private theorem reduce.from_natural
   (hBigStep: conf ==> n): conf.1 conf.2 = n :=
   by induction hBigStep with
-  | add _ _ iha iha' => exact iha.rec $ iha'.rec rfl
-  | sub _ _ iha iha' => exact iha.rec $ iha'.rec rfl
-  | mul _ _ iha iha' => exact iha.rec $ iha'.rec rfl
+  | add _ _ iha iha' => exact iha ▸ iha' ▸ rfl
+  | sub _ _ iha iha' => exact iha ▸ iha' ▸ rfl
+  | mul _ _ iha iha' => exact iha ▸ iha' ▸ rfl
   | _ => rfl
 
 private theorem BigStep.from_reduce
   (hred: a s = n): (a, s) ==> n :=
   by induction a generalizing n with
-  | val a => exact hred.rec BigStep.val
-  | var a => exact hred.rec BigStep.var
+  | val a => exact hred ▸ .val
+  | var a => exact hred ▸ .var
   | add a a' iha iha' =>
-    exact hred.rec (iha rfl).add (iha' rfl)
+    exact hred ▸ (iha rfl).add (iha' rfl)
   | sub a a' iha iha' =>
-    exact hred.rec (iha rfl).sub (iha' rfl)
+    exact hred ▸ (iha rfl).sub (iha' rfl)
   | mul a a' iha iha' =>
-    exact hred.rec (iha rfl).mul (iha' rfl)
+    exact hred ▸ (iha rfl).mul (iha' rfl)
 
 private theorem BigStep_eq_reduce:
   ((a, s) ==> n) = (a s = n) :=
@@ -85,10 +83,10 @@ private theorem BigStep_eq_eq_reduce_eq:
   BigStep.equiv.r b b' <-> reduce.equiv.r b b' := by
   simp only [Setoid.r, eq_iff_iff]
   constructor
-  . exact fun h => Iff.mpr (BigStep_eq_reduce.rec h) (Eq.mpr BigStep_eq_reduce rfl)
+  . exact fun h => Iff.mpr (BigStep_eq_reduce ▸ h) (Eq.mpr BigStep_eq_reduce rfl)
   . exact fun h => {
-      mp := fun h1 => (h ▸ (BigStep_eq_reduce ▸ h1)).rec BigStep_eq_reduce',
-      mpr := fun h1 => (h ▸ (BigStep_eq_reduce ▸ h1)).rec BigStep_eq_reduce'
+      mp := fun h1 => (h ▸ (BigStep_eq_reduce ▸ h1)) ▸ BigStep_eq_reduce',
+      mpr := fun h1 => (h ▸ (BigStep_eq_reduce ▸ h1)) ▸ BigStep_eq_reduce'
     }
 
 end Equivalence
