Semantics/Imp/SmallStep.lean
@@ -4,21 +4,13 @@ import Semantics.ReflTransRel
 namespace Com
 
 inductive SmallStep: Com × State -> Com × State -> Prop where
-  | ass:
-    SmallStep (ass v a, s) (skip, s[v <- a s])
-
-  | skipCat:
-    SmallStep (skip++c, s) (c, s)
-
+  | ass: SmallStep (ass v a, s) (skip, s[v <- a s])
+  | skipCat: SmallStep (skip++c, s) (c, s)
   | cat (hstep: SmallStep (c, s) (c', s')):
     SmallStep (c++c'', s) (c'++c'', s')
-
-  | ifElse:
-    SmallStep (if b then c else c' end, s) (bif b s then c else c', s)
-
+  | ifElse: SmallStep (ifElse b c c', s) (cond (b s) c c', s)
   | whileLoop:
-    SmallStep (while b loop c end, s)
-          (bif b s then c++while b loop c end else skip, s)
+    SmallStep (whileLoop b c, s) (cond (b s) (c++whileLoop b c) skip, s)
 
 infixl:10 " ~> " => SmallStep
 
@@ -26,8 +18,7 @@ namespace SmallStep
 
 private example:
   ([|x := 1; while x <= 2 loop x := x + 1 end|], s0) ~>
-      ([|skip; while x <= 2 loop x := x + 1 end|], s0["x" <- 1]) :=
-  cat ass
+      ([|skip; while x <= 2 loop x := x + 1 end|], s0["x" <- 1]) := cat ass
 
 theorem cat_eq:
   ((c++c'', s) ~> conf)
@@ -42,25 +33,21 @@ theorem cat_eq:
   }
 
 theorem cond_eq:
-  ((if b then c else c' end, s) ~> conf)
-    = (b s ∧ conf = (c, s) ∨ b s = false ∧ conf = (c', s)) :=
-  propext {
+  ((.ifElse b c c', s) ~> conf)
+    = (b s ∧ conf = (c, s) ∨ b s = false ∧ conf = (c', s)) := propext {
     mp := fun hmp => match hb: b s with
       | false => match hmp with | ifElse => Or.inr ⟨rfl, hb ▸ rfl⟩
       | true => match hmp with | ifElse => Or.inl ⟨rfl, hb ▸ rfl⟩,
     mpr := fun hmpr =>
-      let hss: conf = (bif b s then c else c', s) :=
-        match hb: b s with
+      have hss: conf = (cond (b s) c c', s) := match hb: b s with
         | true => match hb ▸ hmpr with | Or.inl ⟨_, hr⟩ => hr
         | false => match hb ▸ hmpr with | Or.inr ⟨_, hr⟩ => hr
       hss ▸ ifElse
   }
 
 theorem cond_false (hb: b s = false):
-  ((if b then c else c' end, s) ~> conf) = (conf = (c', s)) :=
-  propext {
-    mp := fun hmp => match hb ▸ cond_eq ▸ hmp with
-      | Or.inr ⟨_, hr⟩ => hr,
+  ((.ifElse b c c', s) ~> conf) = (conf = (c', s)) := propext {
+    mp := fun hmp => match hb ▸ cond_eq ▸ hmp with | Or.inr ⟨_, hr⟩ => hr,
     mpr := fun mp => cond_eq ▸ Or.inr ⟨hb, mp⟩
   }
 
@@ -78,27 +65,25 @@ private example:
   apply ReflTrans.head (cat ass)
   apply ReflTrans.head skipCat
   apply ReflTrans.head whileLoop
-  have hs : s0["x" <- 1]["x" <- (Aexp.var "x" + 1) (s0["x" <- 1])] = s0["x" <- 1]["x" <- 2] := rfl
-  have hcond : (Bexp.le (Aexp.var "x") 1) (s0["x" <- 1]["x" <- 2]) = false := rfl
+  have hs : s0["x" <- 1]["x" <- (Aexp.var "x" + 1) (s0["x" <- 1])] =
+    s0["x" <- 1]["x" <- 2] := rfl
+  have hcond : (Bexp.le (Aexp.var "x") 1) (s0["x" <- 1]["x" <- 2])
+    = false := rfl
   rw [hs, hcond]
   simp
   apply ReflTrans.refl
 
-theorem star.cat_skip_cat
-  (hc: (c, s) ~>* (skip, s')):
+theorem star.cat_skip_cat (hc: (c, s) ~>* (skip, s')):
   (c++c', s) ~>* (skip++c', s') :=
-  ReflTrans.lift (fun (c, s) => (c++c', s)) (cat .) hc
+  .lift (fun (c, s) => (c++c', s)) (cat .) hc
 
-theorem star.cat
-  (hc: (c, s) ~>* (skip, s'))
-  (hc': (c', s') ~>* (skip, s'')):
+theorem star.cat (hc: (c, s) ~>* (skip, s')) (hc': (c', s') ~>* (skip, s'')):
   (c++c', s) ~>* (skip, s'') :=
-  ReflTrans.trans (cat_skip_cat hc) (ReflTrans.trans (ReflTrans.single skipCat) hc')
+  .trans (cat_skip_cat hc) $ .trans (.single skipCat) hc'
 
-theorem star.cat_no_influence
-  (hc: (c, s) ~>* (skip, s)):
+theorem star.cat_no_influence (hc: (c, s) ~>* (skip, s)):
   (c++c', s) ~>* (c', s) :=
-  ReflTrans.trans (cat_skip_cat hc) (ReflTrans.single skipCat)
+  .trans (cat_skip_cat hc) $ .single skipCat
 
 end SmallStep
 end Com
